theories/base_logic/lib/saved_prop.v
@@ -23,7 +23,7 @@ Section saved_prop.
   Implicit Types x y : F (iProp Σ).
   Implicit Types γ : gname.
 
-  Global Instance saved_prop_persistent γ x : PersistentP (saved_prop_own γ x).
+  Global Instance saved_prop_persistent γ x : Persistent (saved_prop_own γ x).
   Proof. rewrite /saved_prop_own; apply _. Qed.
 
   Lemma saved_prop_alloc_strong x (G : gset gname) :
